Added variants

Evaluate.thy
@@ -1,157 +1,119 @@
 theory Evaluate
-imports Expression Typecheck
+imports Stack
 begin
-
-datatype stack = 
-  SApp1 expr
-| SApp2 expr
-| SRec "expr list" "expr list" 
-| SProj nat
-
-inductive typecheck_stack :: "type list \<Rightarrow> stack list \<Rightarrow> type \<Rightarrow> type \<Rightarrow> bool" 
-    (infix "\<turnstile> _ : _ \<rightarrow>" 60) where
-  tc_hole [simp]: "\<Gamma> \<turnstile> [] : t \<rightarrow> t"
-| tc_sapp1 [simp]: "\<Gamma> \<turnstile> s : t \<rightarrow> Arrow t\<^sub>1 t\<^sub>2 \<Longrightarrow> \<Gamma> \<turnstile> e : t\<^sub>1 \<Longrightarrow> \<Gamma> \<turnstile> SApp1 e # s : t \<rightarrow> t\<^sub>2"
-| tc_sapp2 [simp]: "\<Gamma> \<turnstile> e : Arrow t\<^sub>1 t\<^sub>2 \<Longrightarrow> \<Gamma> \<turnstile> s : t \<rightarrow> t\<^sub>1 \<Longrightarrow> \<Gamma> \<turnstile> SApp2 e # s : t \<rightarrow> t\<^sub>2"
-| tc_srec [simp]: "\<Gamma> \<turnstile>\<^sub>f vs : vts \<Longrightarrow> \<Gamma> \<turnstile>\<^sub>f nvs : nvts \<Longrightarrow> \<Gamma> \<turnstile> s : t \<rightarrow> t' \<Longrightarrow> 
-    \<Gamma> \<turnstile> SRec vs nvs # s : t \<rightarrow> Record (vts @ [t'] @ nvts)"
-| tc_sproj [simp]: "\<Gamma> \<turnstile> s : t \<rightarrow> Record ts \<Longrightarrow> lookup l ts = Some t' \<Longrightarrow> 
-    \<Gamma> \<turnstile> SProj l # s : t \<rightarrow> t'"
-
-fun stack_extend :: "stack \<Rightarrow> stack list \<times> expr \<Rightarrow> stack list \<times> expr" where
-  "stack_extend s' se = (case se of (s, e) \<Rightarrow> (s' # s, e))"
-
-fun unfold :: "expr \<Rightarrow> stack list \<times> expr" 
-and unfold_f :: "expr list \<Rightarrow> expr list \<times> expr list \<times> stack list \<times> expr" where
-  "unfold (Var y) = ([], Var y)"
-| "unfold (Abs t e) = ([], Abs t e)"
-| "unfold (App e\<^sub>1 e\<^sub>2) = (
-    if is_value e\<^sub>1
-    then if is_value e\<^sub>2
-         then ([], App e\<^sub>1 e\<^sub>2)
-         else stack_extend (SApp2 e\<^sub>1) (unfold e\<^sub>2)
-    else stack_extend (SApp1 e\<^sub>2) (unfold e\<^sub>1))"
-| "unfold (Rec fs) = (
-    if is_value_f fs 
-    then ([], Rec fs) 
-    else case unfold_f fs of (vs, nvs, s, e) \<Rightarrow> (SRec vs nvs # s, e))"
-| "unfold (Proj e l) = (
-    if is_value e 
-    then ([], Proj e l) 
-    else stack_extend (SProj l) (unfold e))"
-| "unfold_f [] = undefined"
-| "unfold_f (e # fs) = (
-    if is_value e
-    then case unfold_f fs of (vs, nvs, s, e') \<Rightarrow> (e # vs, nvs, s, e')
-    else ([], fs, unfold e))"
-
-fun fold :: "stack list \<Rightarrow> expr \<Rightarrow> expr" where
-  "fold [] e = e"
-| "fold (SApp1 e' # s) e = App (fold s e) e'"
-| "fold (SApp2 e' # s) e = App e' (fold s e)"
-| "fold (SRec vs nvs # s) e = Rec (vs @ [fold s e] @ nvs)"
-| "fold (SProj l # s) e = Proj (fold s e) l"
 
 inductive reduce :: "expr \<Rightarrow> expr \<Rightarrow> bool" (infix "\<leadsto>\<^sub>\<beta>" 60) where
   ev_beta [simp]: "is_value e\<^sub>2 \<Longrightarrow> App (Abs t e\<^sub>1) e\<^sub>2 \<leadsto>\<^sub>\<beta> subst 0 e\<^sub>2 e\<^sub>1" 
 | ev_proj [simp]: "is_value_f fs \<Longrightarrow> lookup l fs = Some e \<Longrightarrow> Proj (Rec fs) l \<leadsto>\<^sub>\<beta> e" 
+| ev_case [simp]: "is_value e \<Longrightarrow> lookup l cs = Some e' \<Longrightarrow> Case (Inj l ts e) cs \<leadsto>\<^sub>\<beta> subst 0 e e'" 
 
 inductive evaluate :: "expr \<Rightarrow> expr \<Rightarrow> bool" (infix "\<leadsto>" 60) where
   ev_stack [simp]: "unfold e = (s, r) \<Longrightarrow> r \<leadsto>\<^sub>\<beta> r' \<Longrightarrow> e \<leadsto> fold s r'"
 
 inductive_cases [elim]: "e \<leadsto> e'"
 
-lemma [simp]: "unfold e = (s, e') \<Longrightarrow> fold s e' = e"
-  and [simp]: "unfold_f fs = (vs,  nvs, s, e') \<Longrightarrow> \<not> is_value_f fs \<Longrightarrow> 
-    vs @ [fold s e'] @ nvs = fs"
-  by (induction e and fs arbitrary: s e' and vs nvs s e' rule: unfold_unfold_f.induct) 
-     (auto split: if_splits prod.splits)
-
-lemma [simp]: "\<Gamma> \<turnstile> s : t' \<rightarrow> t \<Longrightarrow> \<Gamma> \<turnstile> e : t' \<Longrightarrow> \<Gamma> \<turnstile> fold s e : t"
-  by (induction \<Gamma> s t' t rule: typecheck_stack.induct) simp_all
-
-lemma [simp]: "\<Gamma> \<turnstile> e : t \<Longrightarrow> unfold e = (s, e') \<Longrightarrow> \<exists>t'. (\<Gamma> \<turnstile> s : t' \<rightarrow> t) \<and> (\<Gamma> \<turnstile> e' : t')"
-  and [simp]: "\<Gamma> \<turnstile>\<^sub>f fs : ts \<Longrightarrow> \<not> is_value_f fs \<Longrightarrow> unfold_f fs = (vs, nvs, s, e') \<Longrightarrow> 
-    \<exists>t t' vts nvts. ts = vts @ [t] @ nvts \<and> (\<Gamma> \<turnstile> s : t' \<rightarrow> t) \<and> (\<Gamma> \<turnstile> e' : t') \<and> (\<Gamma> \<turnstile>\<^sub>f vs : vts) \<and> 
-      (\<Gamma> \<turnstile>\<^sub>f nvs : nvts)"
-  proof (induction \<Gamma> e t and \<Gamma> fs ts arbitrary: s and vs nvs s rule: typecheck_typecheck_fs.inducts)
-  case (tc_var x \<Gamma> t)
-    moreover hence "\<Gamma> \<turnstile> Var x : t" by auto
-    ultimately show ?case by force
-  next case (tc_app \<Gamma> e\<^sub>1 t\<^sub>1 t\<^sub>2 e\<^sub>2)
-    thus ?case 
+theorem progress: "[] \<turnstile> e : t \<Longrightarrow> is_value e \<or> (\<exists>e'. e \<leadsto> e')"
+    and "[] \<turnstile>\<^sub>f fs : ts \<Longrightarrow> \<not> is_value_f fs \<Longrightarrow> unfold_f fs = (vs, nvs, s, r) \<Longrightarrow> \<exists>r'. r \<leadsto>\<^sub>\<beta> r'"
+    and "[] \<turnstile>\<^sub>c cs : ts \<rightarrow> t \<Longrightarrow> l < length ts \<Longrightarrow> \<exists>c. lookup l cs = Some c"
+  proof (induction "[] :: type list" e t and "[] :: type list" fs ts and "[] :: type list" cs ts t
+         arbitrary: and vs nvs s r and l
+         rule: typecheck_typecheck_fs_typecheck_cs.inducts)
+  case (tc_app e\<^sub>1 t\<^sub>1 t\<^sub>2 e\<^sub>2)
+    thus ?case
       proof (cases "is_value e\<^sub>1")
       case True note T = True
         thus ?thesis
           proof (cases "is_value e\<^sub>2")
           case True
-            from tc_app have "\<Gamma> \<turnstile> App e\<^sub>1 e\<^sub>2 : t\<^sub>2" by simp
-            with tc_app T True show ?thesis by force
+            moreover from T True have "unfold (App e\<^sub>1 e\<^sub>2) = ([], App e\<^sub>1 e\<^sub>2)" by simp
+            moreover from tc_app T obtain e\<^sub>1' where "e\<^sub>1 = Abs t\<^sub>1 e\<^sub>1'" by fastforce
+            ultimately show ?thesis using ev_stack ev_beta by blast
           next case False
-            with tc_app True obtain s\<^sub>2 where "unfold e\<^sub>2 = (s\<^sub>2, e') \<and> s = SApp2 e\<^sub>1 # s\<^sub>2" 
-              by (auto split: prod.splits)
-            moreover with tc_app obtain t' where "(\<Gamma> \<turnstile> s\<^sub>2 : t' \<rightarrow> t\<^sub>1) \<and> \<Gamma> \<turnstile> e' : t'" by fastforce
-            moreover with tc_app have "\<Gamma> \<turnstile> SApp2 e\<^sub>1 # s\<^sub>2 : t' \<rightarrow> t\<^sub>2" by simp
-            ultimately show ?thesis by fastforce
+            with tc_app obtain s r r' where "unfold e\<^sub>2 = (s, r) \<and> r \<leadsto>\<^sub>\<beta> r' \<and> e\<^sub>2 \<leadsto> fold s r'" 
+              by fastforce
+            moreover with True False have "unfold (App e\<^sub>1 e\<^sub>2) = (SApp2 e\<^sub>1 # s, r)" by simp
+            ultimately show ?thesis using ev_stack by blast
           qed
       next case False
-        with tc_app obtain s\<^sub>1 where "unfold e\<^sub>1 = (s\<^sub>1, e') \<and> s = SApp1 e\<^sub>2 # s\<^sub>1" 
-          by (auto split: prod.splits)
-        moreover with tc_app obtain t' where "(\<Gamma> \<turnstile> s\<^sub>1 : t' \<rightarrow> Arrow t\<^sub>1 t\<^sub>2) \<and> \<Gamma> \<turnstile> e' : t'" 
+        with tc_app obtain s r r' where "unfold e\<^sub>1 = (s, r) \<and> r \<leadsto>\<^sub>\<beta> r' \<and> e\<^sub>1 \<leadsto> fold s r'" 
           by fastforce
-        moreover with tc_app have "\<Gamma> \<turnstile> SApp1 e\<^sub>2 # s\<^sub>1 : t' \<rightarrow> t\<^sub>2" by fastforce
-        ultimately show ?thesis by fastforce
+        moreover with False have "unfold (App e\<^sub>1 e\<^sub>2) = (SApp1 e\<^sub>2 # s, r)" by simp
+        ultimately show ?thesis using ev_stack by blast
       qed
-  next case (tc_abs t\<^sub>1 \<Gamma> e t\<^sub>2)
-    moreover hence "\<Gamma> \<turnstile> Abs t\<^sub>1 e : Arrow t\<^sub>1 t\<^sub>2" by auto
-    ultimately show ?case by force
-  next case (tc_rec \<Gamma> fs ts)
+  next case (tc_rec fs ts)
     thus ?case 
       proof (cases "is_value_f fs")
-      case True
-        moreover with tc_rec have "\<Gamma> \<turnstile> s : Record ts \<rightarrow> Record ts" by simp
-        moreover from tc_rec True have "\<Gamma> \<turnstile> e' : Record ts" by fastforce
-        ultimately show ?thesis by blast
-      next case False
-        then obtain vs nvs ss ee' where F: "unfold_f fs = (vs, nvs, ss, ee')" 
+      case False
+        then obtain vs nvs s e where X: "unfold (Rec fs) = (SRec vs nvs # s, e)" 
           by (cases "unfold_f fs") simp_all
-        with tc_rec False obtain t t' vts nvts where T: "ts = vts @ [t] @ nvts \<and> 
-            (\<Gamma> \<turnstile> ss : t' \<rightarrow> t) \<and> (\<Gamma> \<turnstile> e' : t') \<and> (\<Gamma> \<turnstile>\<^sub>f vs : vts) \<and> \<Gamma> \<turnstile>\<^sub>f nvs : nvts" by fastforce
-        hence "\<Gamma> \<turnstile> SRec vs nvs # ss : t' \<rightarrow> Record ts" using tc_srec by fastforce
-        with tc_rec False F T show ?thesis by fastforce
-      qed
-  next case (tc_proj \<Gamma> e ts l t)
-    thus ?case
+        with False tc_rec obtain e' where "e \<leadsto>\<^sub>\<beta> e'" by (cases "unfold_f fs") fastforce+
+        with X have "Rec fs \<leadsto> fold (SRec vs nvs # s) e'" using ev_stack by fastforce
+        thus ?thesis by fastforce
+      qed simp_all
+  next case (tc_proj e ts l t)
+    thus ?case 
       proof (cases "is_value e")
       case True
-        moreover with tc_proj have "\<Gamma> \<turnstile> s : t \<rightarrow> t" by simp
-        moreover from tc_proj True have "\<Gamma> \<turnstile> e' : t" by fastforce
-        ultimately show ?thesis by blast
+        with tc_proj obtain fs where E: "e = Rec fs \<and> is_value_f fs" by fastforce
+        hence X: "unfold (Proj (Rec fs) l) = ([], Proj (Rec fs) l)" by simp
+        from tc_proj E obtain e' where "lookup l fs = Some e'" by fastforce
+        with E have "Proj (Rec fs) l \<leadsto>\<^sub>\<beta> e'" by simp
+        with X E show ?thesis using ev_stack by fastforce
       next case False
-        with tc_proj obtain ss where "unfold e = (ss, e') \<and> s = SProj l # ss" 
-          by (auto split: prod.splits)
-        moreover with tc_proj obtain t' where "(\<Gamma> \<turnstile> ss : t' \<rightarrow> Record ts) \<and> (\<Gamma> \<turnstile> e' : t')" 
+        with tc_proj obtain s r r' where "unfold e = (s, r) \<and> r \<leadsto>\<^sub>\<beta> r' \<and> e \<leadsto> fold s r'" 
           by fastforce
-        moreover with tc_proj have "\<Gamma> \<turnstile> SProj l # ss : t' \<rightarrow> t" by fastforce
-        ultimately show ?thesis by fastforce
+        moreover with False have "unfold (Proj e l) = (SProj l # s, r)" by simp
+        ultimately show ?thesis using ev_stack by blast
       qed
-  next case (tcf_cons \<Gamma> e tt fs ts)
+  next case (tc_inj e t l ts)
+    thus ?case
+      proof (cases "is_value e")
+      case False
+        with tc_inj obtain s r r' where S: "unfold e = (s, r) \<and> r \<leadsto>\<^sub>\<beta> r' \<and> e \<leadsto> fold s r'" 
+          by fastforce
+        moreover with False have "unfold (Inj l ts e) = (SInj l ts # s, r)" by simp
+        ultimately show ?thesis using ev_stack by blast
+      qed simp_all
+  next case (tc_case e ts cs t)
     thus ?case
       proof (cases "is_value e")
       case True
-        with tcf_cons obtain vs' where V: "unfold_f fs = (vs', nvs, s, e') \<and> vs = e # vs'" 
-          by (cases "unfold_f fs") fastforce+
-        moreover with tcf_cons True obtain t t' vts nvts where T: "ts = vts @ [t] @ nvts \<and> 
-          (\<Gamma> \<turnstile> s : t' \<rightarrow> t) \<and> (\<Gamma> \<turnstile> e' : t') \<and> (\<Gamma> \<turnstile>\<^sub>f vs' : vts) \<and> \<Gamma> \<turnstile>\<^sub>f nvs : nvts" by fastforce
-        moreover hence "tt # ts = (tt # vts) @ [t] @ nvts" by simp
-        moreover from tcf_cons V T have "\<Gamma> \<turnstile>\<^sub>f vs : tt # vts" by simp
-        ultimately show ?thesis by blast
+        with tc_case obtain l e' where E: "e = Inj l ts e' \<and> is_value e' \<and> l < length ts" 
+          by fastforce
+        hence X: "unfold (Case (Inj l ts e') cs) = ([], Case (Inj l ts e') cs)" by simp
+        from tc_case E obtain r' where "lookup l cs = Some r'" by fastforce
+        with E have "Case (Inj l ts e') cs \<leadsto>\<^sub>\<beta> subst 0 e' r'" by simp
+        with X E show ?thesis using ev_stack by fastforce
       next case False
-        with tcf_cons obtain t' where "(\<Gamma> \<turnstile> s : t' \<rightarrow> tt) \<and> \<Gamma> \<turnstile> e' : t'" by fastforce
-        moreover from tcf_cons False have "\<Gamma> \<turnstile>\<^sub>f vs : []" by simp
-        moreover from tcf_cons False have "\<Gamma> \<turnstile>\<^sub>f nvs : ts" by simp
-        ultimately show ?thesis by fastforce
+        with tc_case obtain s r r' where S: "unfold e = (s, r) \<and> r \<leadsto>\<^sub>\<beta> r' \<and> e \<leadsto> fold s r'" 
+          by fastforce
+        moreover with False have "unfold (Case e cs) = (SCase cs # s, r)" by simp
+        ultimately show ?thesis using ev_stack by blast
       qed
+  next case (tcf_cons e t fs ts l)
+    thus ?case
+      proof (cases "is_value e")
+      case True
+        with tcf_cons show ?thesis by (cases "unfold_f fs") simp_all
+      qed fastforce+
+  next case (tcc_cons t' e t fs ts)
+    thus ?case by (induction l) simp_all
   qed simp_all
+
+lemma preservation\<^sub>\<beta>: "e \<leadsto>\<^sub>\<beta> e' \<Longrightarrow> \<Gamma> \<turnstile> e : t \<Longrightarrow> \<Gamma> \<turnstile> e' : t"
+  proof (induction e e' rule: reduce.induct) 
+  case (ev_case e l cs e' ts)
+    then obtain t' where "(\<Gamma> \<turnstile> e : t') \<and> lookup l ts = Some t' \<and> \<Gamma> \<turnstile>\<^sub>c cs : ts \<rightarrow> t" by fastforce
+    moreover with ev_case have "insert_at 0 t' \<Gamma> \<turnstile> e' : t" by fastforce
+    ultimately show ?case by simp
+  qed fastforce+
+
+theorem preservation: "e \<leadsto> e' \<Longrightarrow> \<Gamma> \<turnstile> e : t \<Longrightarrow> \<Gamma> \<turnstile> e' : t"
+  proof (induction e e' rule: evaluate.induct)
+  case (ev_stack e s r r')
+    then obtain t' where "(\<Gamma> \<turnstile> s : t' \<rightarrow> t) \<and> \<Gamma> \<turnstile> r : t'" by fastforce
+    moreover with ev_stack have "\<Gamma> \<turnstile> r' : t'" using preservation\<^sub>\<beta> by simp
+    ultimately show ?case by fastforce
+  qed
 
 end
