Expression.thy
@@ -6,6 +6,7 @@ datatype type =
   Base
 | Arrow type type
 | Record "type list"
+| Variant "type list"
 
 datatype expr = 
   Var nat
@@ -13,6 +14,8 @@ datatype expr =
 | App expr expr
 | Rec "expr list"
 | Proj expr nat
+| Inj nat "type list" expr
+| Case expr "expr list"
 
 primrec incr :: "nat \<Rightarrow> expr \<Rightarrow> expr" where
   "incr x (Var y) = Var (if x \<le> y then Suc y else y)"
@@ -20,6 +23,8 @@ primrec incr :: "nat \<Rightarrow> expr \<Rightarrow> expr" where
 | "incr x (App e\<^sub>1 e\<^sub>2) = App (incr x e\<^sub>1) (incr x e\<^sub>2)"
 | "incr x (Rec fs) = Rec (map (incr x) fs)"
 | "incr x (Proj e l) = Proj (incr x e) l"
+| "incr x (Inj l ts e) = Inj l ts (incr x e)"
+| "incr x (Case e cs) = Case (incr x e) (map (incr (Suc x)) cs)"
 
 primrec subst :: "nat \<Rightarrow> expr \<Rightarrow> expr \<Rightarrow> expr" where
   "subst x e' (Var y) = (if x = y then e' else Var (if x < y then y - 1 else y))"
@@ -27,6 +32,8 @@ primrec subst :: "nat \<Rightarrow> expr \<Rightarrow> expr \<Rightarrow> expr" 
 | "subst x e' (App e\<^sub>1 e\<^sub>2) = App (subst x e' e\<^sub>1) (subst x e' e\<^sub>2)"
 | "subst x e' (Rec fs) = Rec (map (subst x e') fs)"
 | "subst x e' (Proj e l) = Proj (subst x e' e) l"
+| "subst x e' (Inj l ts e) = Inj l ts (subst x e' e)"
+| "subst x e' (Case e cs) = Case (subst x e' e) (map (subst (Suc x) (incr 0 e')) cs)"
 
 primrec is_value :: "expr \<Rightarrow> bool" 
     and is_value_f :: "expr list \<Rightarrow> bool" where
@@ -35,6 +42,8 @@ primrec is_value :: "expr \<Rightarrow> bool"
 | "is_value (App e\<^sub>1 e\<^sub>2) = False"
 | "is_value (Rec fs) = is_value_f fs"
 | "is_value (Proj e l) = False"
+| "is_value (Inj l ts e) = is_value e"
+| "is_value (Case e cs) = False"
 | "is_value_f [] = True"
 | "is_value_f (e # fs) = (is_value e \<and> is_value_f fs)"
 
