Stack.thy
@@ -1,0 +1,191 @@
+theory Stack
+imports Typecheck
+begin
+
+datatype stack = 
+  SApp1 expr
+| SApp2 expr
+| SRec "expr list" "expr list" 
+| SProj nat
+| SInj nat "type list"
+| SCase "expr list" 
+
+inductive typecheck_stack :: "type list \<Rightarrow> stack list \<Rightarrow> type \<Rightarrow> type \<Rightarrow> bool" 
+    (infix "\<turnstile> _ : _ \<rightarrow>" 60) where
+  tc_hole [simp]: "\<Gamma> \<turnstile> [] : t \<rightarrow> t"
+| tc_sapp1 [simp]: "\<Gamma> \<turnstile> s : t \<rightarrow> Arrow t\<^sub>1 t\<^sub>2 \<Longrightarrow> \<Gamma> \<turnstile> e : t\<^sub>1 \<Longrightarrow> \<Gamma> \<turnstile> SApp1 e # s : t \<rightarrow> t\<^sub>2"
+| tc_sapp2 [simp]: "\<Gamma> \<turnstile> e : Arrow t\<^sub>1 t\<^sub>2 \<Longrightarrow> \<Gamma> \<turnstile> s : t \<rightarrow> t\<^sub>1 \<Longrightarrow> \<Gamma> \<turnstile> SApp2 e # s : t \<rightarrow> t\<^sub>2"
+| tc_srec [simp]: "\<Gamma> \<turnstile>\<^sub>f vs : vts \<Longrightarrow> \<Gamma> \<turnstile>\<^sub>f nvs : nvts \<Longrightarrow> \<Gamma> \<turnstile> s : t \<rightarrow> t' \<Longrightarrow> 
+    \<Gamma> \<turnstile> SRec vs nvs # s : t \<rightarrow> Record (vts @ [t'] @ nvts)"
+| tc_sproj [simp]: "\<Gamma> \<turnstile> s : t \<rightarrow> Record ts \<Longrightarrow> lookup l ts = Some t' \<Longrightarrow> 
+    \<Gamma> \<turnstile> SProj l # s : t \<rightarrow> t'"
+| tc_sinj [simp]: "\<Gamma> \<turnstile> s : t \<rightarrow> t' \<Longrightarrow> lookup l ts = Some t' \<Longrightarrow> \<Gamma> \<turnstile> SInj l ts # s : t \<rightarrow> Variant ts"
+| tc_scase [simp]: "\<Gamma> \<turnstile> s : t \<rightarrow> Variant ts \<Longrightarrow> \<Gamma> \<turnstile>\<^sub>c cs : ts \<rightarrow> t' \<Longrightarrow> \<Gamma> \<turnstile> SCase cs # s : t \<rightarrow> t'"
+
+fun stack_extend :: "stack \<Rightarrow> stack list \<times> expr \<Rightarrow> stack list \<times> expr" where
+  "stack_extend s' se = (case se of (s, e) \<Rightarrow> (s' # s, e))"
+
+fun unfold :: "expr \<Rightarrow> stack list \<times> expr" 
+and unfold_f :: "expr list \<Rightarrow> expr list \<times> expr list \<times> stack list \<times> expr" where
+  "unfold (Var y) = ([], Var y)"
+| "unfold (Abs t e) = ([], Abs t e)"
+| "unfold (App e\<^sub>1 e\<^sub>2) = (
+    if is_value e\<^sub>1
+    then if is_value e\<^sub>2
+         then ([], App e\<^sub>1 e\<^sub>2)
+         else stack_extend (SApp2 e\<^sub>1) (unfold e\<^sub>2)
+    else stack_extend (SApp1 e\<^sub>2) (unfold e\<^sub>1))"
+| "unfold (Rec fs) = (
+    if is_value_f fs 
+    then ([], Rec fs) 
+    else case unfold_f fs of (vs, nvs, s, e) \<Rightarrow> (SRec vs nvs # s, e))"
+| "unfold (Proj e l) = (
+    if is_value e 
+    then ([], Proj e l) 
+    else stack_extend (SProj l) (unfold e))"
+| "unfold (Inj l ts e) = (
+    if is_value e 
+    then ([], Inj l ts e) 
+    else stack_extend (SInj l ts) (unfold e))"
+| "unfold (Case e cs) = (
+    if is_value e 
+    then ([], Case e cs) 
+    else stack_extend (SCase cs) (unfold e))"
+| "unfold_f [] = undefined"
+| "unfold_f (e # fs) = (
+    if is_value e
+    then case unfold_f fs of (vs, nvs, s, e') \<Rightarrow> (e # vs, nvs, s, e')
+    else ([], fs, unfold e))"
+
+fun fold :: "stack list \<Rightarrow> expr \<Rightarrow> expr" where
+  "fold [] e = e"
+| "fold (SApp1 e' # s) e = App (fold s e) e'"
+| "fold (SApp2 e' # s) e = App e' (fold s e)"
+| "fold (SRec vs nvs # s) e = Rec (vs @ [fold s e] @ nvs)"
+| "fold (SProj l # s) e = Proj (fold s e) l"
+| "fold (SInj l ts # s) e = Inj l ts (fold s e)"
+| "fold (SCase cs # s) e = Case (fold s e) cs"
+
+lemma [simp]: "unfold e = (s, e') \<Longrightarrow> fold s e' = e"
+  and [simp]: "unfold_f fs = (vs,  nvs, s, e') \<Longrightarrow> \<not> is_value_f fs \<Longrightarrow> 
+    vs @ [fold s e'] @ nvs = fs"
+  by (induction e and fs arbitrary: s e' and vs nvs s e' rule: unfold_unfold_f.induct) 
+     (auto split: if_splits prod.splits)
+
+lemma [simp]: "\<Gamma> \<turnstile> s : t' \<rightarrow> t \<Longrightarrow> \<Gamma> \<turnstile> e : t' \<Longrightarrow> \<Gamma> \<turnstile> fold s e : t"
+  by (induction \<Gamma> s t' t rule: typecheck_stack.induct) simp_all
+
+lemma [simp]: "\<Gamma> \<turnstile> e : t \<Longrightarrow> unfold e = (s, e') \<Longrightarrow> \<exists>t'. (\<Gamma> \<turnstile> s : t' \<rightarrow> t) \<and> (\<Gamma> \<turnstile> e' : t')"
+  and [simp]: "\<Gamma> \<turnstile>\<^sub>f fs : ts \<Longrightarrow> \<not> is_value_f fs \<Longrightarrow> unfold_f fs = (vs, nvs, s, e') \<Longrightarrow> 
+    \<exists>t t' vts nvts. ts = vts @ [t] @ nvts \<and> (\<Gamma> \<turnstile> s : t' \<rightarrow> t) \<and> (\<Gamma> \<turnstile> e' : t') \<and> (\<Gamma> \<turnstile>\<^sub>f vs : vts) \<and> 
+      (\<Gamma> \<turnstile>\<^sub>f nvs : nvts)"
+  and [simp]: "\<Gamma> \<turnstile>\<^sub>c cs : ts \<rightarrow> t \<Longrightarrow> True"
+  proof (induction \<Gamma> e t and \<Gamma> fs ts arbitrary: s and vs nvs s 
+         rule: typecheck_typecheck_fs_typecheck_cs.inducts)
+  case (tc_var x \<Gamma> t)
+    moreover hence "\<Gamma> \<turnstile> Var x : t" by auto
+    ultimately show ?case by force
+  next case (tc_app \<Gamma> e\<^sub>1 t\<^sub>1 t\<^sub>2 e\<^sub>2)
+    thus ?case 
+      proof (cases "is_value e\<^sub>1")
+      case True note T = True
+        thus ?thesis
+          proof (cases "is_value e\<^sub>2")
+          case True
+            from tc_app have "\<Gamma> \<turnstile> App e\<^sub>1 e\<^sub>2 : t\<^sub>2" by simp
+            with tc_app T True show ?thesis by force
+          next case False
+            with tc_app True obtain s\<^sub>2 where "unfold e\<^sub>2 = (s\<^sub>2, e') \<and> s = SApp2 e\<^sub>1 # s\<^sub>2" 
+              by (auto split: prod.splits)
+            moreover with tc_app obtain t' where "(\<Gamma> \<turnstile> s\<^sub>2 : t' \<rightarrow> t\<^sub>1) \<and> \<Gamma> \<turnstile> e' : t'" by fastforce
+            moreover with tc_app have "\<Gamma> \<turnstile> SApp2 e\<^sub>1 # s\<^sub>2 : t' \<rightarrow> t\<^sub>2" by simp
+            ultimately show ?thesis by fastforce
+          qed
+      next case False
+        with tc_app obtain s\<^sub>1 where "unfold e\<^sub>1 = (s\<^sub>1, e') \<and> s = SApp1 e\<^sub>2 # s\<^sub>1" 
+          by (auto split: prod.splits)
+        moreover with tc_app obtain t' where "(\<Gamma> \<turnstile> s\<^sub>1 : t' \<rightarrow> Arrow t\<^sub>1 t\<^sub>2) \<and> \<Gamma> \<turnstile> e' : t'" 
+          by fastforce
+        moreover with tc_app have "\<Gamma> \<turnstile> SApp1 e\<^sub>2 # s\<^sub>1 : t' \<rightarrow> t\<^sub>2" by fastforce
+        ultimately show ?thesis by fastforce
+      qed
+  next case (tc_abs t\<^sub>1 \<Gamma> e t\<^sub>2)
+    moreover hence "\<Gamma> \<turnstile> Abs t\<^sub>1 e : Arrow t\<^sub>1 t\<^sub>2" by auto
+    ultimately show ?case by force
+  next case (tc_rec \<Gamma> fs ts)
+    thus ?case 
+      proof (cases "is_value_f fs")
+      case True
+        moreover with tc_rec have "\<Gamma> \<turnstile> s : Record ts \<rightarrow> Record ts" by simp
+        moreover from tc_rec True have "\<Gamma> \<turnstile> e' : Record ts" by fastforce
+        ultimately show ?thesis by blast
+      next case False
+        then obtain vs nvs ss ee' where F: "unfold_f fs = (vs, nvs, ss, ee')" 
+          by (cases "unfold_f fs") simp_all
+        with tc_rec False obtain t t' vts nvts where T: "ts = vts @ [t] @ nvts \<and> 
+            (\<Gamma> \<turnstile> ss : t' \<rightarrow> t) \<and> (\<Gamma> \<turnstile> e' : t') \<and> (\<Gamma> \<turnstile>\<^sub>f vs : vts) \<and> \<Gamma> \<turnstile>\<^sub>f nvs : nvts" by fastforce
+        hence "\<Gamma> \<turnstile> SRec vs nvs # ss : t' \<rightarrow> Record ts" using tc_srec by fastforce
+        with tc_rec False F T show ?thesis by fastforce
+      qed
+  next case (tc_proj \<Gamma> e ts l t)
+    thus ?case
+      proof (cases "is_value e")
+      case True
+        moreover with tc_proj have "\<Gamma> \<turnstile> s : t \<rightarrow> t" by simp
+        moreover from tc_proj True have "\<Gamma> \<turnstile> e' : t" by fastforce
+        ultimately show ?thesis by blast
+      next case False
+        with tc_proj obtain ss where "unfold e = (ss, e') \<and> s = SProj l # ss" 
+          by (auto split: prod.splits)
+        moreover with tc_proj obtain t' where "(\<Gamma> \<turnstile> ss : t' \<rightarrow> Record ts) \<and> (\<Gamma> \<turnstile> e' : t')" 
+          by fastforce
+        moreover with tc_proj have "\<Gamma> \<turnstile> SProj l # ss : t' \<rightarrow> t" by fastforce
+        ultimately show ?thesis by fastforce
+      qed
+  next case (tc_inj \<Gamma> e t l ts)
+    thus ?case
+      proof (cases "is_value e")
+      case True
+        from tc_inj have "\<Gamma> \<turnstile> Inj l ts e : Variant ts" by simp
+        with tc_inj True show ?thesis by force
+      next case False
+        with tc_inj obtain s' where S: "unfold e = (s', e') \<and> s = SInj l ts # s'" 
+          by (auto split: prod.splits)
+        with tc_inj obtain t' where "(\<Gamma> \<turnstile> s' : t' \<rightarrow> t) \<and> (\<Gamma> \<turnstile> e' : t')" by fastforce
+        moreover with tc_inj S have "\<Gamma> \<turnstile> s : t' \<rightarrow> Variant ts" using tc_sinj by fastforce
+        ultimately show ?thesis by fastforce
+      qed
+  next case (tc_case \<Gamma> e ts cs t)
+    thus ?case
+      proof (cases "is_value e")
+      case True
+        with tc_case have "\<Gamma> \<turnstile> s : t \<rightarrow> t" by simp
+        moreover from tc_case True have "\<Gamma> \<turnstile> e' : t" by fastforce
+        ultimately show ?thesis by fastforce
+      next case False
+        with tc_case obtain s' where S: "unfold e = (s', e') \<and> s = SCase cs # s'" 
+          by (auto split: prod.splits)
+        with tc_case obtain t' where T: "(\<Gamma> \<turnstile> s' : t' \<rightarrow> Variant ts) \<and> (\<Gamma> \<turnstile> e' : t')" by fastforce
+        with tc_case S have "\<Gamma> \<turnstile> s : t' \<rightarrow> t" using tc_scase by fastforce
+        with T show ?thesis by fastforce
+      qed
+  next case (tcf_cons \<Gamma> e tt fs ts)
+    thus ?case
+      proof (cases "is_value e")
+      case True
+        with tcf_cons obtain vs' where V: "unfold_f fs = (vs', nvs, s, e') \<and> vs = e # vs'" 
+          by (cases "unfold_f fs") fastforce+
+        moreover with tcf_cons True obtain t t' vts nvts where T: "ts = vts @ [t] @ nvts \<and> 
+          (\<Gamma> \<turnstile> s : t' \<rightarrow> t) \<and> (\<Gamma> \<turnstile> e' : t') \<and> (\<Gamma> \<turnstile>\<^sub>f vs' : vts) \<and> \<Gamma> \<turnstile>\<^sub>f nvs : nvts" by fastforce
+        moreover hence "tt # ts = (tt # vts) @ [t] @ nvts" by simp
+        moreover from tcf_cons V T have "\<Gamma> \<turnstile>\<^sub>f vs : tt # vts" by simp
+        ultimately show ?thesis by blast
+      next case False
+        with tcf_cons obtain t' where "(\<Gamma> \<turnstile> s : t' \<rightarrow> tt) \<and> \<Gamma> \<turnstile> e' : t'" by fastforce
+        moreover from tcf_cons False have "\<Gamma> \<turnstile>\<^sub>f vs : []" by simp
+        moreover from tcf_cons False have "\<Gamma> \<turnstile>\<^sub>f nvs : ts" by simp
+        ultimately show ?thesis by fastforce
+      qed
+  qed simp_all
+
+end
